thys/Buchi_Complementation/Ranking.thy
@@ -103,7 +103,7 @@ begin
       using assms unfolding ranking_def by auto
     have 9: "\<And> p. p \<in> sset (gtrace ?t ?u) \<Longrightarrow> gaccepting A p \<Longrightarrow> even (f p)" using 7 8 by auto
 
-    have 19: "infs (accepting A) (smap snd ?r)" using 2(3) unfolding trace_alt_def by simp
+    have 19: "infs (accepting A) (smap snd ?r)" using 2(3) unfolding nba.trace_alt_def by simp
     have 18: "infs (gaccepting A) ?r" using 19 by simp
     have 17: "infs (gaccepting A) (gtrace ?r ?v)" using 18 unfolding gtrace_alt_def by this
     have 16: "infs (gaccepting A) (gtrace (?s @- ?t) ?v)" using 17 unfolding stake_sdrop by this
@@ -237,7 +237,7 @@ begin
     have 91: "sset (trace (w ||| s) q) \<subseteq> reachable A q"
       using nba.reachable_trace nba.reachable.reflexive 8 by this
     have 10: "fins (accepting A) (trace (w ||| s) q)" using 3 9 8 by this
-    have 11: "fins (accepting A) s" using 10 unfolding trace_alt_def by simp
+    have 11: "fins (accepting A) s" using 10 unfolding nba.trace_alt_def by simp
     have 12: "infs (gaccepting A) r" using infs_mono[OF _ 6(2)] by simp
     have "s = smap snd (t @- y @- r)" unfolding 7(1) by simp
     also have "infs (accepting A) \<dots>" using 12 by (simp add: comp_def)
