thys/Transition_Systems_and_Automata/Automata/NBA/NBA_Algorithms.thy
@@ -33,7 +33,7 @@ begin
     lemma nba_g_ahs: "nba_g A = \<lparr> g_V = UNIV, g_E = E_of_succ (\<lambda> p. CAST
       ((\<Union> a \<in> alphabet A. transition A a p ::: \<langle>S\<rangle> list_set_rel) ::: \<langle>S\<rangle> ahs_rel bhc)),
       g_V0 = initial A \<rparr>"
-      unfolding nba_g_def successors_alt_def CAST_def id_apply autoref_tag_defs by rule
+      unfolding nba_g_def nba.successors_alt_def CAST_def id_apply autoref_tag_defs by rule
 
     schematic_goal nbai_gi:
       notes [autoref_ga_rules] = map2set_to_list
@@ -81,7 +81,7 @@ begin
     lemma nba_igbg_ahs: "nba_igbg A = \<lparr> g_V = UNIV, g_E = E_of_succ (\<lambda> p. CAST
       ((\<Union> a \<in> alphabet A. transition A a p ::: \<langle>S\<rangle> list_set_rel) ::: \<langle>S\<rangle> ahs_rel bhc)), g_V0 = initial A,
       igbg_num_acc = 1, igbg_acc = \<lambda> p. if accepting A p then {0} else {} \<rparr>"
-      unfolding nba_g_def nba_igbg_def successors_alt_def CAST_def id_apply autoref_tag_defs
+      unfolding nba_g_def nba_igbg_def nba.successors_alt_def CAST_def id_apply autoref_tag_defs
       unfolding graph_rec.defs
       by simp
 
